# lecture 
## Equations and Expressions


### Equations

- **Definition:** Equations are mathematical statements indicating that two expressions are equal.
- **Solvability:** Equations can be solved to find the value of the variable(s) that make the equation true.
    - Example: 3x = 9
    - The '=' sign denotes balance, indicating that both sides of the equation are equal.

### Expressions

- **Definition:** Expressions are mathematical phrases that may contain variables, constants, and operations but do not have an equal sign.
- **Solvability:** Expressions cannot be solved as they lack the balance provided by the equal sign.
    - Example: 4x + 7

### Simple Linear Equations

- **Characteristics:** Simple linear equations involve a single variable raised to the first power.
- **Solvability:** They follow a straightforward process and require no complex thought to solve.

#### Process:

1.  **One-Step Process:**
    
    - Example: x + 2 = 3
    - Subtract 2 from both sides to keep it balanced:  
        x + 2 - 2 = 3 - 2
    - Result: x = 1
2.  **Another Example:**
    
    - x - 4 = 3
    - Add 4 to both sides to maintain balance:  
        x - 4 + 4 = 3 + 4
    - Result: x = 7
3.  **Division:**
    
    - 2x = 4
    - Divide both sides by 2 to keep balance:  
        2x/2 = 4/2
    - Result: x = 2
4.  **Multiplication:**
    
    - x/3 = 1
    - Multiply both sides by 3 to maintain balance:  
        x/3 \* 3 = 1 \* 3
    - Result: x = 3

#### Multiple Steps

- **Example 1:**
    
    - 2x + 3 = 9
    - Isolate the term including x by subtracting 3 from both sides:  
        2x + 3 - 3 = 9 - 3
    - Divide by 2:  
        2x/2 = 6/2
    - Result: x = 3
- **Example 2 (With Decimals):**
    
    - 2.4x + 3.6 = 9.9
    - Isolate the term including x by subtracting 3.6 from both sides:  
        2.4x + 3.6 - 3.6 = 9.9 - 3.6
    - Divide by 2.4:  
        2.4x/2.4 = 6.3/2.4
    - Result: x = 2.625
- **Example 3 (More Processes):**
    
    - 2x/3 + 4 = 12
    - Subtract 4 from both sides:  
        2x/3 + 4 - 4 = 12 -4
    - Multiply by 3:  
        2x/3 \* 3 = 8 \* 3
    - Divide by 2:  
        2x/2 = 24/2
    - Result: x = 12

#### Simplifying Equations

- **Definition:** Simple equations have the variable occur only once.
- **Example:**
    - (4x + 3 = 2)
    - Some equations could be like this if they were simplified:  
        (2x + 3 + 4x + 4 = x - 8 + 5)
    - On each side, the numbers are combined, and the x terms are combined:  
        ((2x + 4x) + (3 + 4) = x + (-8 + 5))
    - Simplify further:  
        (6x + 7 = x - 3)
    - Then, remove letters from one side and numbers from the other:  
        (6x - x + 7 = x - x - 3)  
        (5x + 7 = -3)  
        (5x + 7 - 7 = -3 -7)  
        (5x = -10)  
        (x = -2)

#### Revision Questions

- **Question 1:**
    
    - (4y - 7 = 21)
    - (4y - 7 + 7 = 21 + 7)
    - (4y = 28)
    - (4y/4 = 28/4)
    - (y = 7)
- **Question 2:**
    
    - (2x + 4 = 5x - 2)
    - (2x + 4 - 4 = 4x -2 -4)
    - (2x = 5x - 6)
    - (2x - 5x = 5x - 6 - 5x)
    - (-3x = -6)
    - (-3x/3 = -6/3)
    - (x = 2)
- **Question 3:**
    
    - (7x + 3 = 4x - 3 + x + 6)
    - (7x + 3 = 4x + 3 + x)
    - (7x + 3 = 5x + 3)
    - (7x + 3 - 3 = 5x + 3 - 3)
    - (7x = 5x)
    - (7x - 5x = 5x -5x)
    - (2x = 0)
    - (2x/2 = 0/2)
    - (x = 0/2)
    - (x = 0)
- **Question 4:**
    
    - (x² + x - 7 = x² + 2)
    - (x² + x - 7 - (x² + 2) = 0)
    - (x² + x -7 - x² - 2 = 0)
    - (x² + x - 9 - x² = 0)
    - (x - 9 = 0)
    - (x - 9 + 9 = 0 + 9)
    - (x = 9)

## Brackets

multiplying a singlebracekt  
2(x + 3)  
2 \* x + 2 \* 3  
2x + 6

x(x - 4)  
x \* x + x \* x \* -4  
x² - 4x

\-3(x + 1)  
\-3 \* x + -3 \* 1  
\-3x - 3

\-2(x - 2)  
\-2 \* x - 2 \* -2  
\-2x + 4

Highest Common Factor  
HCF is largest factor in both numbers'

24 =  
1 \* 24  
2 \* 24  
3 \* 8  
4 \* 6

18=  
1 \* 18  
2 \* 9  
3 \* 6  
HCF of 18 and 24 is 6

Lowest common multiple  
to the lcm you multiply the two numbers together and divide by the HCF  
24 \* 18 / 6 = 72  
24, 48, 72, 96  
18, 36, 54, 72, 90

factorising by finding common factors

2x + 10 HCF = 2  
2 \* x + 2 \* 5  
2(x + 5)

6x - 15 HCF = 3  
3 \* 2x - 3 \* 5  
3(2x - 5)

x² + 2x HCF = x  
x \* x + x + 2  
x(x + 2)

3x² + 9x HCF = 3x  
3x \* x + 3x \* 3  
3x(x + 3)

Questions

7(x + 4)  
7 \* x + 7 \* 4  
7x + 28

x(2 - x)  
x \* 2 - x \* x  
2x - x²

5x + 20 HCF =5  
5 \* x + 4 \* 5  
5(x + 4)

x² + 2x HCF = x  
x \* x + x \* 2  
x(x + 2)

2x² - 8x HCF = 2x  
2x \* x - 2x \* 4  
2x(x - 4)

Rearranging formulae  
Formulae  
like equations but with letters instead of numbers  
x + t = g  
g would be the subject  
When rearranging we want to make a different letter the subject  
for example to make x the subject subtact t  
x + t - t = g - t  
x = g - t

just like simple linear equations  
theres a process to follow  
equations with letters in place of numbers  
making x the subject means solving to find x  
x + 2 = 3 -> x = 1  
x + a = b -> b -a

x - 1 = 5 -> x = 6  
x - c = d -> x + d + c

2x = 4 -> x = 2  
ex = f -> x = f/e

Making x the subject

ax = p  
divide by a  
ax/a = p/a  
x = p/a

x/q = r  
multiply by q  
x/q \* q = r \* q  
x = rq

cx + d = e  
subtract the d  
cx + d - d = e - d  
cx = d - e  
cx/c = d - e/c

f(x + g) = h  
divide by f  
f(x + g)/f =h/f  
x + g = h/f  
Subtract the g  
x + g - g = h/f - g  
x = h/f - g

Questions

tx - q = z  
tx - q + q = z + q  
tx = q + z  
tx/t = q + z/t  
x = q + z/t

rx - w = j + k  
rx - w + w = j + k + w  
rx = j + k + w  
rx/r = j + k/r + w  
x = j + k + w/r

ax/b = c  
ax/b \* b = c \* b  
ax = cb  
ax/a = cb/a  
x = cb/a

g(x/h + m) = p  
g(x/h + m)/g = p/g  
x/h + m = p/g  
x/h + m - m = p/g - m  
x/h = p/g - m  
x/h \* h = p/h - m \* h  
x = h(p/g - m)

Simultaneous equations

Multiple varibles  
two letters requires 2 equations  
x + y = 3  
x - y = 1  
two answers for soulotion  
solve as a pair

x + y = 3  
x - y = 1  
eliminate y  
signs different so add equations  
x + x = 2x  
y - y = 0  
3 + 1 = 4  
2x = 4  
x = 2

Subsitiute x into either equation to find y  
x + y = 3  
2 + y = 3  
y = 1  
or  
x - y = 1  
2 - y = 1  
y = 1

3x + 2y = 25  
2x + 2y = 18  
eliminate y  
signs the same so subtract  
3x - 2x = xx  
2y - 2y = 0  
25 - 18 = 7  
x = 7  
Subsitiute x into either equation to find y  
3x + 2y = 25  
(3 * 7) + 2y = 25  
21 + 2y = 25  
y = 2

2x + 4y = 2  
3x + 2y = 11  
eliminate y but the values are different  
multiply second equation by 2  
6x - 4y = 22  
2x + 6x = 8x  
4y + -4y = 0  
2 + 22 = 24  
8x = 24  
x = 3  
Subsitiute x into either equation to find y  
2x + 4 = 2  
(2 \* 3) + 4y = 2  
6 + 4y = 2  
y = -1

7x + 2y = 70  
5x + 9y = 50  
eliminate y but values different  
multiply first equation by 9  
63x + 18y = 630  
10x + 18y = 100  
63x - 10x = 53x  
18y - 18y = 0  
630 - 100 = 530  
53x = 530  
x = 10  
7x + 2y = 70  
(7 \* 10) + 2y = 70  
70 + 2y = 70  
y = 0
